RelationalAlgebra/RA/EquivRules.lean
@@ -6,7 +6,7 @@ open RM
 @[simp ←]
 theorem projection_union {s' : RelationSchema} (inst1 inst2 : RelationInstance) (h_pr : s' ⊆ inst1.schema) (h_un : inst1.schema = inst2.schema):
   projection (union inst1 inst2 h_un) s' h_pr = union (projection inst1 s' h_pr) (projection inst2 s' (by rw [←h_un]; exact h_pr)) rfl := by
-    unfold projection union
+    unfold projection union projectionT unionT
     simp_all only [Set.mem_union, RelationInstance.mk.injEq, true_and]
     ext x : 1
     simp_all only [Set.mem_setOf_eq, Set.mem_union]
